src/lib/inst/Kuiper.DotProduct.fsti
@@ -1,0 +1,11 @@
+module Kuiper.DotProduct
+
+#lang-pulse
+
+open Kuiper
+module P = Kuiper.Poly.DotProduct
+
+val dotprod_f32 : P.dotprod_ty f32
+val dotprod_f64 : P.dotprod_ty f64
+val dotprod_u32 : P.dotprod_ty u32
+val dotprod_u64 : P.dotprod_ty u64
